Tactics.v
@@ -1,0 +1,3 @@
+Ltac inv H := inversion H; subst; simpl; auto.
+
+Ltac contra := intros top; contradiction top; clear top.
